Add new notation

dimsum/iris/expr2.v
@@ -25,9 +25,30 @@ Global Arguments mtrans {_ _} _.
 Global Arguments mexpr_rel {_ _} _ _ _.
 Global Arguments mstate_interp {_ _} _ _.
 
+
+(* NOTE - This is actually a little  *)
+Definition sim_gen_mapsto_state `{!dimsumGS Σ} {EV} (ts : tgt_src) (m : mod_trans EV)
+  (H_s : (m_state m) → (option EV → m_state m → iProp Σ) → iProp Σ) : iProp Σ :=
+  ∀ σ Π, H_s σ Π -∗ σ ≈{ts, m}≈> Π.
+Notation "PΠ '⥥{' ts , m '}'" := (sim_gen_mapsto_state ts m PΠ)
+  (at level 20, only parsing) : bi_scope.
+
+Notation "PΠ '⥥{' ts '}'" := (sim_gen_mapsto_state ts _ PΠ)
+  (at level 20, format "PΠ '⥥{' ts '}'") : bi_scope.
+Notation "PΠ '⥥{' m '}ₜ'" := (sim_gen_mapsto_state Tgt m PΠ)
+  (at level 20, only parsing) : bi_scope.
+Notation "PΠ '⥥ₜ'" := (sim_gen_mapsto_state Tgt _ PΠ)
+  (at level 20, format "PΠ '⥥ₜ'") : bi_scope.
+
+Notation "PΠ '⥥{' m '}ₛ'" := (sim_gen_mapsto_state Src m PΠ)
+  (at level 20, only parsing) : bi_scope.
+Notation "PΠ '⥥ₛ'" := (sim_gen_mapsto_state Src _  PΠ)
+  (at level 20, format "PΠ '⥥ₛ'") : bi_scope.
+
 Definition switch `{!dimsumGS Σ} {S EV} (Π : option EV → S → iProp Σ)
   (K : option EV → S → (tgt_src → ∀ EV2, ∀ m : mod_trans EV2, _ → iProp Σ) → iProp Σ) : iProp Σ :=
-  (∀ κ σ, K κ σ (λ ts' EV2 m' PΠ', ∀ σ' Π', PΠ' σ' Π' -∗ σ' ≈{ ts', m' }≈> Π') -∗  Π κ σ).
+  (∀ κ σ, K κ σ (λ ts' EV2 m' PΠ', PΠ' ⥥{ts', m'}) -∗  Π κ σ).
+  (* (∀ κ σ, K κ σ (λ ts' EV2 m' PΠ', ∀ σ' Π', PΠ' σ' Π' -∗ σ' ≈{ ts', m' }≈> Π') -∗  Π κ σ). *)
 
 (* Lemma switch_mono `{!dimsumGS Σ} {S EV} (Π : option EV → S → iProp Σ) K1 K2 : *)
 (*   switch Π K1 -∗ *)
@@ -128,7 +149,7 @@ Section sim_gen_expr.
   Proof.
     move => ?? Hsim ?? -> ?? HΦ. rewrite /sim_gen_expr_pre.
     repeat (f_equiv || eapply Hsim || eapply HΦ || reflexivity).
-    move => ?? -> ?? ->. unfold switch_id, curly_lambda2, curly_lambda3, switch.
+    move => ?? -> ?? ->. unfold switch_id, curly_lambda2, curly_lambda3, switch, sim_gen_mapsto_state.
     repeat (f_equiv || eapply Hsim || eapply HΦ || reflexivity).
   Qed.
 
